destrci

thy/Conc_Impl.thy
@@ -20,6 +20,11 @@ definition "ifci v t e bdd \<equiv> (if t = e then return (t, bdd) else do {
 	(p,u) \<leftarrow> pointermap_getmki (v, t, e) bdd;
 	return (Suc (Suc p), u)
 })"
+definition destrci :: "nat \<Rightarrow> (nat \<times> nat \<times> nat) pointermap_impl \<Rightarrow> (nat, nat) IFEXD Heap" where
+"destrci n bdd \<equiv> (case n of
+	0 \<Rightarrow> return FD |
+	Suc 0 \<Rightarrow> return TD |
+	Suc (Suc p) \<Rightarrow> pm_pthi bdd p \<guillemotright>= (\<lambda>lu. case lu of (v,t,e) \<Rightarrow> return (IFD v t e)))"
 
 lemma [sep_heap_rules]: "<is_pointermap_impl bdd bddi> tci bddi <\<lambda>r. is_pointermap_impl bdd (snd r) * \<up>(fst r = fst (tmi bdd))>"
 by(sep_auto simp: tci_def)
@@ -29,6 +34,11 @@ lemma [sep_heap_rules]: "(p, u) = ifmi v t e bdd \<Longrightarrow>
 	<is_pointermap_impl bdd bddi> ifci v t e bddi
 	<\<lambda>(pi,ui). is_pointermap_impl u ui * \<up>(pi = p)>\<^sub>t"
 by(sep_auto simp: ifci_def apfst_def map_prod_def split: prod.splits if_splits)
+lemma [sep_heap_rules]: "
+	n < 2 \<or> pointermap_p_valid (n - 2) bdd \<Longrightarrow>
+	<is_pointermap_impl bdd bddi> destrci n bddi
+	<\<lambda>r. is_pointermap_impl bdd bddi * \<up>(r = destrmi n bdd)>\<^sub>t"
+by(cases "(n, bdd)" rule: destrmi.cases) (sep_auto simp: destrci_def)+
 
 
 end
